src/coq/Semantics/Memory/MemBytes.v
@@ -10,7 +10,8 @@ From Vellvm Require Import
      Semantics.LLVMEvents
      Utils.Monads
      Utils.NMaps
-     Utils.OptionUtil.
+     Utils.OptionUtil
+     Utils.ListUtil.
 
 Import Basics.Basics.Monads.
 
@@ -51,6 +52,7 @@ Module Byte(Addr:ADDRESS)(SIZEOF:Sizeof)(LLVMEvents:LLVM_INTERACTIONS(Addr)(SIZE
   Export Byte.
   Import LLVMEvents.
   Import DV.
+  Import SIZEOF.
 
   Fixpoint all_bytes_from_uvalue_helper (idx' : Z) (sid' : store_id) (parent : uvalue) (bytes : list SByte) : option uvalue
     := match bytes with
@@ -76,4 +78,46 @@ Module Byte(Addr:ADDRESS)(SIZEOF:Sizeof)(LLVMEvents:LLVM_INTERACTIONS(Addr)(SIZE
          | _ => None
          end
        end.
+
+  Definition to_ubytes (uv :  uvalue) (dt : dtyp) (sid : store_id) : list SByte
+    := map (fun n => uvalue_sbyte uv dt (UVALUE_IPTR (Z.of_N n)) sid) (Nseq 0 (N.to_nat (sizeof_dtyp dt))).
+
+  Fixpoint all_extract_bytes_from_uvalue_helper (idx' : Z) (sid' : store_id) (dt' : dtyp) (parent : uvalue) (bytes : list uvalue) : option uvalue
+    := match bytes with
+       | [] => Some parent
+       | (UVALUE_ExtractByte uv dt idx sid)::bytes =>
+         guard_opt (uvalue_int_eq_Z idx idx');;
+         guard_opt (RelDec.rel_dec uv parent);;
+         guard_opt (N.eqb sid sid');;
+         guard_opt (dtyp_eqb dt dt');;
+         all_extract_bytes_from_uvalue_helper (Z.succ idx') sid' dt' parent bytes
+       | _ => None
+       end.
+
+  (* Check that store ids, uvalues, and types match up, as well as
+       that the extract byte indices are in the right order *)
+  Definition all_extract_bytes_from_uvalue (bytes : list uvalue) : option uvalue
+    := match bytes with
+       | nil => None
+       | (UVALUE_ExtractByte uv dt idx sid)::xs =>
+         all_extract_bytes_from_uvalue_helper 0 sid dt uv bytes
+       | _ => None
+       end.
+
+  Definition from_ubytes (bytes : list SByte) (dt : dtyp) : uvalue
+    :=
+      match N.eqb (N.of_nat (length bytes)) (sizeof_dtyp dt), all_bytes_from_uvalue bytes with
+      | true, Some uv => uv
+      | _, _ => UVALUE_ConcatBytes (map sbyte_to_extractbyte bytes) dt
+      end.
+
+  Lemma to_ubytes_sizeof :
+    forall uv dt sid,
+      N.of_nat (length (to_ubytes uv dt sid)) = sizeof_dtyp dt.
+  Proof.
+    intros uv dt sid.
+    unfold to_ubytes.
+    rewrite map_length. rewrite Nseq_length.
+    apply Nnat.N2Nat.id.
+  Qed.
 End Byte.
