src/coq/Handlers/FiniteMemoryTheory.v
@@ -45,6 +45,7 @@ From Vellvm Require Import
      Semantics.Memory.Sizeof
      Semantics.Memory.MemBytes
      Semantics.Memory.ErrSID
+     Handlers.SerializationTheory
      Semantics.GepM
      Semantics.LLVMEvents
      Handlers.FiniteMemory.
@@ -86,6 +87,11 @@ Module Type MEMORY_THEORY (SIZE:Sizeof)(LLVMEvents: LLVM_INTERACTIONS(Addr)(SIZE
   Module ESID := ERRSID Addr SIZE LLVMEvents PROV.
   Import ESID.
 
+  Module MBT := MemBytesTheory Addr SIZE LLVMEvents PTOI PROV ITOP GEP BYTE_IMPL.
+  Import MBT.
+
+  Module ST := SerializationTheory SIZE LLVMEvents PTOI PROV ITOP GEP BYTE_IMPL.
+  Import ST.
 
   (* TODO: move this? *)
   Definition ErrSID_evals_to {A} (e : ErrSID A) sid pr (x : A) : Prop
@@ -260,16 +266,6 @@ Section Serialization_Theory.
   (*   intros dt dts. *)
   (*   rewrite fold_sum_acc. reflexivity. *)
   (* Qed. *)
-
-  Lemma to_ubytes_sizeof :
-    forall uv dt sid,
-      N.of_nat (length (to_ubytes uv dt sid)) = sizeof_dtyp dt.
-  Proof.
-    intros uv dt sid.
-    unfold to_ubytes.
-    rewrite map_length. rewrite Nseq_length.
-    apply Nnat.N2Nat.id.
-  Qed.
 
   Lemma sizeof_serialized :
     forall uv dt sid prov bytes,
@@ -543,9 +539,14 @@ Section Serialization_Theory.
       intros bytes bytes' sid prov EVAL.
       induction bytes.
       - inv EVAL; auto.
-      - cbn in EVAL.
+      - red in EVAL.
+        unfold evalErrSID in EVAL.
+        unfold IdentityMonad.unIdent in EVAL.
+        unfold evalErrSID_T in EVAL.
+        unfold re_sid_ubytes in EVAL.
+        cbn in EVAL.
     Admitted.
-    
+
     apply ErrSID_evals_to_bind in BYTES as (sid'' & prov'' & bytes'' & EXTRACT & BYTES).
 
     Lemma map_monad_lift_ERR :
@@ -670,7 +671,7 @@ Section Serialization_Theory.
   apply map_monad_ErrSID_length in EXTRACT.
   apply re_sid_ubytes_ErrSID_length in BYTES.
   lia.
-  Qed.
+  Admitted.
 
   (* Lemma firstn_sizeof_dtyp : *)
   (*   forall dv dt, *)
@@ -1367,531 +1368,7 @@ Section Memory_Stack_Theory.
     (*     replace (Datatypes.length elt_bytes + 0)%nat with (Datatypes.length elt_bytes) by lia. *)
     (*     rewrite skipn_length_app. *)
     (*     congruence. *)
-    (* Qed. *)
-
-Lemma all_bytes_helper_app :
-  forall  sbytes sbytes2 start sid uv,
-    all_bytes_from_uvalue_helper (Z.of_N start) sid uv sbytes = Some uv ->
-    all_bytes_from_uvalue_helper (Z.of_N (start + N.of_nat (length sbytes))) sid uv sbytes2 = Some uv ->
-    all_bytes_from_uvalue_helper (Z.of_N start) sid uv (sbytes ++ sbytes2) = Some uv.
-Proof.
-  induction sbytes;
-    intros sbytes2 start sid uv INIT REST.
-  - now rewrite N.add_0_r in REST.
-  - cbn.
-    destruct a.
-    cbn in INIT.
-    do 3 (break_match; [|solve [inv INIT]]).
-
-
-    cbn in REST. auto.
-    replace (Z.of_N (start + N.pos (Pos.of_succ_nat (Datatypes.length sbytes)))) with (Z.of_N (N.succ start + N.of_nat (Datatypes.length sbytes))) in REST by lia.
-
-    rewrite <- N2Z.inj_succ in *.
-    
-    apply IHsbytes; auto.
-Qed.
-
-Lemma to_ubytes_all_bytes_from_uvalue_helper' :
-  forall len uv dt sid sbytes start,
-    is_supported dt ->
-    map (fun n : N => UByte uv dt (UVALUE_IPTR (Z.of_N n)) sid) (Nseq start len) = sbytes ->
-    all_bytes_from_uvalue_helper (Z.of_N start) sid uv sbytes = Some uv.
-Proof.
-  induction len;
-    intros uv dt sid sbytes start SUP TO.
-  - inv TO; reflexivity.
-  - inv TO.
-    rewrite Nseq_S.
-    rewrite map_app.
-    apply all_bytes_helper_app; eauto.
-    + cbn.
-      rewrite map_length.
-      rewrite Nseq_length.
-      solve_guards_all_bytes.
-      reflexivity.
-Qed.
-
-Lemma to_ubytes_all_bytes_from_uvalue_helper :
-  forall uv dt sid sbytes,
-    is_supported dt ->
-    to_ubytes uv dt sid = sbytes ->
-    all_bytes_from_uvalue_helper 0 sid uv sbytes = Some uv.
-Proof.  
-  intros uv dt sid sbytes SUP TO.
-
-  change 0%Z with (Z.of_N 0).
-  eapply to_ubytes_all_bytes_from_uvalue_helper'; eauto.    
-Qed.
-
-Lemma to_ubytes_sizeof_dtyp :
-  forall uv dt sid,  
-    N.of_nat (length (to_ubytes uv dt sid)) = sizeof_dtyp dt.
-Proof.
-  intros uv dt sid.
-  unfold to_ubytes.
-  rewrite map_length, Nseq_length.
-  lia.
-Qed.
-
-Lemma from_ubytes_to_ubytes :
-  forall uv dt sid,
-    is_supported dt ->
-    sizeof_dtyp dt > 0 ->
-    from_ubytes (to_ubytes uv dt sid) dt = uv.
-Proof.
-  intros uv dt sid SUP SIZE.
-
-  unfold from_ubytes.
-  unfold all_bytes_from_uvalue.
-
-  rewrite to_ubytes_sizeof_dtyp.
-  rewrite N.eqb_refl.
-
-  break_inner_match.
-  - (* Contradiction by size *)
-    pose proof to_ubytes_sizeof_dtyp uv dt sid.
-    rewrite Heql in H.
-
-    cbn in *.
-    lia.
-  - destruct s.
-    cbn in *.
-
-    unfold to_ubytes in Heql.
-    remember (sizeof_dtyp dt) as sz.
-    destruct sz; [inv SIZE|].
-    cbn in *.
-    pose proof Pos2Nat.is_succ p as [sz Hsz].
-    rewrite Hsz in Heql.
-    rewrite <- cons_Nseq in Heql.
-
-    cbn in Heql.
-    inv Heql.
-    cbn.
-
-    solve_guards_all_bytes.
-
-    cbn.
-    change 1%Z with (Z.of_N 1).
-    erewrite to_ubytes_all_bytes_from_uvalue_helper'; eauto.
-Qed.
-
-Lemma serialize_sbytes_deserialize_sbytes :
-  forall uv dt sid sbytes ,
-    uvalue_has_dtyp uv dt ->
-    is_supported dt ->
-    sizeof_dtyp dt > 0 ->
-    evalErrSID (serialize_sbytes uv dt) sid = inr (sbytes) ->
-    deserialize_sbytes sbytes dt = inr uv.
-Proof.
-  intros uv dt sid sbytes TYP SUP SIZE SER.
-  induction TYP;
-    try solve [unfold serialize_sbytes in SER;
-               inv SER;
-               unfold deserialize_sbytes;
-               rewrite from_ubytes_to_ubytes; eauto
-              | cbn in *;
-                match goal with
-                | |- deserialize_sbytes _ ?t = _ =>
-                  cbn in *;
-                  destruct t; cbn; inv SER;
-                  rewrite from_ubytes_to_ubytes; eauto
-                end
-              ].
-  - inv SUP; exfalso; apply H; constructor.
-  - rewrite sizeof_dtyp_void in SIZE. inv SIZE.
-Qed.
-
-
-    (** ** Deserialize - Serialize
-        Starting from a dvalue [val] whose [dtyp] is [t], if:
-        1. we serialize [val], getting a [list SByte]
-        2. we add all these bytes to the memory block, starting from the position [off], getting back a new [mem_block] m'
-        3. we lookup in this new memory [m'] the indices starting from [off] for the size of [t], getting back a [list SByte]
-        4. we deserialize this final list of bytes
-        then we should get back the initial value [val], albeit injected into [uvalue].
-
-        The proof should go by induction over [TYP] I think, and rely on [lookup_all_index_add] notably.
-     *)
-    Lemma deserialize_serialize : forall val dt sid prov bytes,
-        uvalue_has_dtyp val dt ->
-        ErrSID_evals_to (serialize_sbytes val dt) sid prov bytes ->
-        deserialize_sbytes bytes dt = inr val.
-    Proof.
-      intros val dt sid prov bytes TYP SER.
-      induction TYP.
-      - cbn in SER; inv SER.
-        cbn.
-        rewrite 
-    Qed.
-
-    
-    (* Lemma deserialize_serialize : forall val t (TYP : dvalue_has_dtyp val t), *)
-    (*     forall off (bytes : mem_block) (SUP : is_supported t), *)
-    (*       deserialize_sbytes (lookup_all_index off (sizeof_dtyp t) (add_all_index (serialize_dvalue val) off bytes) SUndef) t = dvalue_to_uvalue val. *)
-    (* Proof. *)
-    (*   induction 1; try auto; intros; *)
-    (*     match goal with *)
-    (*     | H: is_supported ?t |- _ => *)
-    (*       try solve [inversion H] *)
-    (*     end. *)
-    (*   - unroll_lookup_all_index; cbn; f_equal. *)
-    (*   - unroll_lookup_all_index; cbn; f_equal. *)
-    (*     pose proof (unsigned_I1_in_range x). *)
-    (*     assert (EQ :DynamicValues.Int1.unsigned x / 256 = 0). *)
-    (*     apply Z.div_small; lia. *)
-    (*     rewrite EQ. *)
-    (*     repeat rewrite Zdiv_0_l. *)
-    (*     repeat rewrite Byte.unsigned_repr. *)
-    (*     all: unfold Byte.max_unsigned, Byte.modulus; cbn; try lia. *)
-    (*     rewrite Z.add_0_r. *)
-    (*     apply DynamicValues.Int1.repr_unsigned. *)
-    (*   - solve_integer_deserialize. *)
-    (*   - solve_integer_deserialize. *)
-    (*   - solve_integer_deserialize. *)
-    (*   - inversion SUP; subst; *)
-    (*     exfalso; apply H; constructor. *)
-    (*   - unroll_lookup_all_index; cbn; f_equal. *)
-    (*     clear bytes off. *)
-    (*     remember (Float.to_bits x) as xb. *)
-    (*     pose proof (unsigned_I64_in_range xb). *)
-    (*     repeat rewrite Byte.unsigned_repr_eq. *)
-    (*     unfold Byte.modulus, Byte.wordsize, Wordsize_8.wordsize; cbn. *)
-    (*     replace (two_power_nat 8) with 256 by reflexivity. *)
-    (*     remember (Int64.unsigned xb) as xbv. *)
-    (*     match goal with *)
-    (*     | [|- context[Int64.repr ?zv]] => replace zv with xbv *)
-    (*     end. *)
-    (*     + *)
-    (*       subst. *)
-    (*       rewrite Int64.repr_unsigned. *)
-    (*       apply Float.of_to_bits. *)
-    (*     + *)
-    (*       (* this is the same goal as I64 branch! *) *)
-    (*       clear -H. *)
-    (*       rewrite Z.add_0_r. *)
-    (*       unfold Z.modulo. *)
-    (*       repeat break_let. *)
-    (*       repeat match goal with *)
-    (*              | [H : Z.div_eucl _ _ = _ |- _] => apply Z_div_mod' in H; [destruct H | lia] *)
-    (*              end. *)
-    (*       subst. *)
-    (*       repeat *)
-    (*         match goal with *)
-    (*         | H: context [(?d * ?x + ?z) / ?d] |- _ => *)
-    (*           rewrite div_add_lemma in H; [|lia]; subst *)
-    (*         end. *)
-    (*       lia. *)
-    (*   - unroll_lookup_all_index; cbn; f_equal. *)
-    (*     clear bytes off. *)
-    (*     remember (Float32.to_bits x) as xb. *)
-    (*     pose proof (unsigned_I32_in_range xb). *)
-    (*     repeat rewrite Byte.unsigned_repr_eq. *)
-    (*     unfold Byte.modulus, Byte.wordsize, Wordsize_8.wordsize; cbn. *)
-    (*     replace (two_power_nat 8) with 256 by reflexivity. *)
-    (*     remember (Int32.unsigned xb) as xbv. *)
-    (*     match goal with *)
-    (*     | [|- context[Int32.repr ?zv]] => replace zv with xbv *)
-    (*     end. *)
-    (*     + *)
-    (*       subst. *)
-    (*       rewrite Int32.repr_unsigned. *)
-    (*       apply Float32.of_to_bits. *)
-    (*     + *)
-    (*       clear -H. *)
-
-    (*       rewrite Z.add_0_r. *)
-    (*       unfold Z.modulo. *)
-    (*       repeat break_let. *)
-    (*       repeat match goal with *)
-    (*              | [H : Z.div_eucl _ _ = _ |- _] => apply Z_div_mod' in H; [destruct H | lia] *)
-    (*              end. *)
-    (*       subst. *)
-    (*       rewrite Z.add_comm, Z.mul_comm, Z_div_plus in * by lia. *)
-    (*       rewrite Zdiv_small with (x:=z0) in * by lia. *)
-    (*       rewrite Z.add_0_l in *. *)
-    (*       subst. *)
-    (*       rewrite Z.add_comm, Z.mul_comm, Z_div_plus in * by lia. *)
-    (*       rewrite Zdiv_small with (x:=z2) in * by lia. *)
-    (*       rewrite Z.add_0_l in *. *)
-    (*       subst. *)
-    (*       rewrite Z.add_comm, Z.mul_comm, Z_div_plus in * by lia. *)
-    (*       rewrite Zdiv_small with (x:=z4) in * by lia. *)
-    (*       rewrite Z.add_0_l in *. *)
-    (*       subst. *)
-    (*       lia. *)
-    (*   - (* Structs *) *)
-    (*     rewrite sizeof_struct_cons. *)
-
-    (*     inversion SUP. *)
-    (*     subst. *)
-    (*     rename H0 into FIELD_SUP. *)
-    (*     apply List.Forall_cons_iff in FIELD_SUP. *)
-    (*     destruct FIELD_SUP as [dt_SUP dts_SUP]. *)
-    (*     assert (is_supported (DTYPE_Struct dts)) as SUP_STRUCT by (constructor; auto). *)
-
-    (*     cbn. *)
-    (*     rewrite lookup_all_index_append; [|apply sizeof_serialized; auto]. *)
-
-    (*     erewrite deserialize_struct_element; auto. *)
-    (*     +  erewrite <- sizeof_serialized; eauto. *)
-    (*       rewrite lookup_all_index_add_all_index_same_length; eauto. *)
-
-    (*       apply dvalue_serialized_not_sundef. *)
-    (*     + pose proof deserialize_sbytes_dvalue_all_not_sundef (DVALUE_Struct fields) (DTYPE_Struct dts) (lookup_all_index (off + Z.of_N (sizeof_dtyp dt)) (sizeof_dtyp (DTYPE_Struct dts)) *)
-    (*                                                                                                                       (add_all_index (serialize_dvalue (DVALUE_Struct fields)) (off + Z.of_N (sizeof_dtyp dt)) bytes) SUndef). *)
-    (*       cbn in H. *)
-    (*       forward H; auto. *)
-    (*     + rewrite lookup_all_index_length. *)
-    (*       reflexivity. *)
-    (*   - (* Packed structs *) *)
-    (*     rewrite sizeof_packed_struct_cons. *)
-
-    (*     inversion SUP. *)
-    (*     subst. *)
-    (*     rename H0 into FIELD_SUP. *)
-    (*     apply List.Forall_cons_iff in FIELD_SUP. *)
-    (*     destruct FIELD_SUP as [dt_SUP dts_SUP]. *)
-    (*     assert (is_supported (DTYPE_Packed_struct dts)) as SUP_STRUCT by (constructor; auto). *)
-
-    (*     cbn. *)
-    (*     rewrite lookup_all_index_append; [|apply sizeof_serialized; auto]. *)
-
-    (*     erewrite deserialize_packed_struct_element; auto. *)
-    (*     + erewrite <- sizeof_serialized; eauto. *)
-    (*       rewrite lookup_all_index_add_all_index_same_length; eauto. *)
-
-    (*       apply dvalue_serialized_not_sundef. *)
-    (*     + pose proof deserialize_sbytes_dvalue_all_not_sundef (DVALUE_Packed_struct fields) (DTYPE_Packed_struct dts) (lookup_all_index (off + Z.of_N (sizeof_dtyp dt)) (sizeof_dtyp (DTYPE_Packed_struct dts)) *)
-    (*                                                                                                                       (add_all_index (serialize_dvalue (DVALUE_Packed_struct fields)) (off + Z.of_N (sizeof_dtyp dt)) bytes) SUndef). *)
-    (*       cbn in H. *)
-    (*       forward H; auto. *)
-    (*     + rewrite lookup_all_index_length. *)
-    (*       reflexivity. *)
-    (*   - (* Arrays *) *)
-    (*     rename H into SZ. *)
-    (*     generalize dependent sz. *)
-    (*     generalize dependent xs. *)
-    (*     induction xs; *)
-    (*       intros IH IHdtyp sz SZ SUP. *)
-    (*     + cbn in *. *)
-    (*       subst. *)
-    (*       reflexivity. *)
-    (*     + cbn in SZ. *)
-    (*       subst. *)
-    (*       rewrite Nnat.Nat2N.inj_succ. *)
-    (*       cbn. *)
-
-    (*       assert (dvalue_has_dtyp a dt) as DTa. *)
-    (*       { *)
-    (*         apply IHdtyp. *)
-    (*         cbn. auto. *)
-    (*       } *)
-
-    (*       rewrite Nmult_Sn_m. *)
-    (*       rewrite lookup_all_index_append; [|apply sizeof_serialized; auto]. *)
-
-    (*       erewrite deserialize_array_element; auto. *)
-    (*       * inversion SUP; constructor; auto. *)
-    (*       * erewrite <- sizeof_serialized; eauto. *)
-    (*         rewrite lookup_all_index_add_all_index_same_length; eauto. *)
-
-    (*         apply dvalue_serialized_not_sundef. *)
-    (*       * (* Should be serialization of DVALUE_array xs *) *)
-    (*         replace (N.of_nat (Datatypes.length xs) * sizeof_dtyp dt)%N *)
-    (*           with (N.of_nat (N.to_nat (N.of_nat (Datatypes.length xs) * sizeof_dtyp dt))) by lia. *)
-    (*         rewrite lookup_all_index_add_all_index_same_length. *)
-
-    (*         apply all_not_sundef_fold_right_serialize. *)
-
-    (*         apply serialize_fold_length; intuition. *)
-    (*       * replace (sizeof_dtyp dt) with (N.of_nat (N.to_nat (sizeof_dtyp dt))) by lia. *)
-    (*         rewrite lookup_all_index_add_all_index_same_length. *)
-    (*         erewrite <- sizeof_serialized; intuition. *)
-    (*         lia. *)
-    (*         erewrite <- sizeof_serialized; intuition. *)
-    (*         lia. *)
-    (*       * rewrite IH; intuition. *)
-    (*         inversion SUP; auto. *)
-    (*       * cbn. *)
-
-    (*         unfold deserialize_sbytes. *)
-    (*         break_match. *)
-
-    (*         2: { *)
-    (*           assert (all_not_sundef *)
-    (*                     (lookup_all_index (off + Z.of_N (sizeof_dtyp dt)) *)
-    (*                                       (N.of_nat (Datatypes.length xs) * sizeof_dtyp dt) *)
-    (*                                       (add_all_index *)
-    (*                                          (fold_right (fun (dv : dvalue) (acc : list SByte) => serialize_dvalue dv ++ acc) [] *)
-    (*                                                      xs) (off + Z.of_N (sizeof_dtyp dt)) bytes) SUndef) = true) as CONTRA. *)
-    (*           replace (N.of_nat (Datatypes.length xs) * sizeof_dtyp dt)%N *)
-    (*             with (N.of_nat (N.to_nat (N.of_nat (Datatypes.length xs) * sizeof_dtyp dt))) by lia. *)
-    (*           rewrite lookup_all_index_add_all_index_same_length. *)
-
-    (*           apply all_not_sundef_fold_right_serialize. *)
-
-    (*           apply serialize_fold_length; intuition. *)
-
-    (*           rewrite Heqb in CONTRA. *)
-    (*           inversion CONTRA. *)
-    (*         } *)
-
-    (*         forward IHxs; intuition. *)
-    (*         forward IHxs; intuition. *)
-    (*         specialize (IHxs (Datatypes.length xs) eq_refl). *)
-    (*         forward IHxs. *)
-    (*         { inversion SUP; constructor; eauto. } *)
-
-    (*         cbn in IHxs. *)
-    (*         rewrite <- IHxs. *)
-
-    (*         rewrite all_not_sundef_deserialized; auto. *)
-    (*         erewrite <- sizeof_serialized. *)
-
-    (*         f_equal. *)
-
-    (*         repeat rewrite <- Nnat.Nat2N.inj_mul. *)
-    (*         rewrite lookup_all_index_add_all_index_same_length. *)
-    (*         rewrite lookup_all_index_add_all_index_same_length. *)
-    (*         reflexivity. *)
-
-    (*         { erewrite <- serialize_fold_length. *)
-    (*           erewrite <- sizeof_serialized. *)
-
-    (*           repeat rewrite <- Nnat.Nat2N.inj_mul. *)
-    (*           rewrite Nnat.Nat2N.id. *)
-    (*           reflexivity. *)
-
-    (*           eauto. *)
-    (*           intuition. *)
-    (*         } *)
-
-    (*         { erewrite <- serialize_fold_length. *)
-    (*           erewrite <- sizeof_serialized. *)
-
-    (*           repeat rewrite <- Nnat.Nat2N.inj_mul. *)
-    (*           rewrite Nnat.Nat2N.id. *)
-    (*           reflexivity. *)
-
-    (*           eauto. *)
-    (*           intuition. *)
-    (*         } *)
-
-    (*         eauto. *)
-    (*   - (* Vectors *) *)
-    (*     rename H into SZ. *)
-    (*     generalize dependent sz. *)
-    (*     generalize dependent xs. *)
-    (*     induction xs; *)
-    (*       intros IH IHdtyp sz SZ SUP. *)
-    (*     + cbn in *. *)
-    (*       subst. *)
-    (*       reflexivity. *)
-    (*     + cbn in SZ. *)
-    (*       subst. *)
-    (*       rewrite Nnat.Nat2N.inj_succ. *)
-    (*       cbn. *)
-
-    (*       assert (dvalue_has_dtyp a dt) as DTa. *)
-    (*       { *)
-    (*         apply IHdtyp. *)
-    (*         cbn. auto. *)
-    (*       } *)
-
-    (*       rewrite Nmult_Sn_m. *)
-    (*       rewrite lookup_all_index_append; [|apply sizeof_serialized; auto]. *)
-
-    (*       erewrite deserialize_vector_element; auto. *)
-    (*       * inversion SUP; constructor; auto. *)
-    (*       * erewrite <- sizeof_serialized; eauto. *)
-    (*         rewrite lookup_all_index_add_all_index_same_length; eauto. *)
-
-    (*         apply dvalue_serialized_not_sundef. *)
-    (*       * (* Should be serialization of DVALUE_vector xs *) *)
-    (*         replace (N.of_nat (Datatypes.length xs) * sizeof_dtyp dt)%N *)
-    (*           with (N.of_nat (N.to_nat (N.of_nat (Datatypes.length xs) * sizeof_dtyp dt))) by lia. *)
-    (*         rewrite lookup_all_index_add_all_index_same_length. *)
-
-    (*         apply all_not_sundef_fold_right_serialize. *)
-
-    (*         apply serialize_fold_length; intuition. *)
-    (*       * replace (sizeof_dtyp dt) with (N.of_nat (N.to_nat (sizeof_dtyp dt))) by lia. *)
-    (*         rewrite lookup_all_index_add_all_index_same_length. *)
-    (*         erewrite <- sizeof_serialized; intuition. *)
-    (*         lia. *)
-    (*         erewrite <- sizeof_serialized; intuition. *)
-    (*         lia. *)
-    (*       * rewrite IH; intuition. *)
-    (*         inversion SUP; subst; auto. *)
-    (*       * cbn. *)
-
-    (*         unfold deserialize_sbytes. *)
-    (*         break_match. *)
-
-    (*         2: { *)
-    (*           assert (all_not_sundef *)
-    (*                     (lookup_all_index (off + Z.of_N (sizeof_dtyp dt)) *)
-    (*                                       (N.of_nat (Datatypes.length xs) * sizeof_dtyp dt) *)
-    (*                                       (add_all_index *)
-    (*                                          (fold_right (fun (dv : dvalue) (acc : list SByte) => serialize_dvalue dv ++ acc) [] *)
-    (*                                                      xs) (off + Z.of_N (sizeof_dtyp dt)) bytes) SUndef) = true) as CONTRA. *)
-    (*           replace (N.of_nat (Datatypes.length xs) * sizeof_dtyp dt)%N *)
-    (*             with (N.of_nat (N.to_nat (N.of_nat (Datatypes.length xs) * sizeof_dtyp dt))) by lia. *)
-    (*           rewrite lookup_all_index_add_all_index_same_length. *)
-
-    (*           apply all_not_sundef_fold_right_serialize. *)
-
-    (*           apply serialize_fold_length; intuition. *)
-
-    (*           rewrite Heqb in CONTRA. *)
-    (*           inversion CONTRA. *)
-    (*         } *)
-
-    (*         forward IHxs; intuition. *)
-    (*         forward IHxs; intuition. *)
-    (*         specialize (IHxs (Datatypes.length xs) eq_refl). *)
-    (*         forward IHxs. *)
-    (*         { inversion SUP; constructor; eauto. } *)
-
-    (*         cbn in IHxs. *)
-    (*         rewrite <- IHxs. *)
-
-    (*         rewrite all_not_sundef_deserialized; auto. *)
-    (*         erewrite <- sizeof_serialized. *)
-
-    (*         f_equal. *)
-
-    (*         repeat rewrite <- Nnat.Nat2N.inj_mul. *)
-    (*         rewrite lookup_all_index_add_all_index_same_length. *)
-    (*         rewrite lookup_all_index_add_all_index_same_length. *)
-    (*         reflexivity. *)
-
-    (*         { erewrite <- serialize_fold_length. *)
-    (*           erewrite <- sizeof_serialized. *)
-
-    (*           repeat rewrite <- Nnat.Nat2N.inj_mul. *)
-    (*           rewrite Nnat.Nat2N.id. *)
-    (*           reflexivity. *)
-
-    (*           eauto. *)
-    (*           intuition. *)
-    (*         } *)
-
-    (*         { erewrite <- serialize_fold_length. *)
-    (*           erewrite <- sizeof_serialized. *)
-
-    (*           repeat rewrite <- Nnat.Nat2N.inj_mul. *)
-    (*           rewrite Nnat.Nat2N.id. *)
-    (*           reflexivity. *)
-
-    (*           eauto. *)
-    (*           intuition. *)
-    (*         } *)
-
-    (*         eauto. *)
-    (* Qed. *)
+    (* Qed. *)    
 
     (* (** ** Write - Read *)
     (*     The expected law: reading the key that has just been written to returns the written value. *)
@@ -3169,6 +2646,11 @@ Section PARAMS.
       cbn.
       repeat rewrite bind_ret_l.
       cbn.
+      (* Can I avoid this rewriting? *)
+      unfold ErrSID_MemState_ms_runs_to in Hwrite.
+      unfold Mem.ESID.runErrSID.
+      unfold runErrSID in Hwrite.
+      unfold runErrSID_T, Mem.ESID.runErrSID_T in *.
       rewrite Hwrite.
       repeat rewrite bind_ret_l; cbn.
       destruct m, m'; cbn.
