src/coq/Handlers/SerializationTheory.v
@@ -16,7 +16,7 @@ From Vellvm Require Import
      Semantics.Memory.MemBytes
      Semantics.Memory.ErrSID.
 
-Module MemBytesTheory(Addr:MemoryAddress.ADDRESS)(LLVMIO: LLVM_INTERACTIONS(Addr))(SIZEOF: Sizeof)(PTOI:PTOI(Addr))(PROVENANCE:PROVENANCE(Addr))(ITOP:ITOP(Addr)(PROVENANCE))(GEP:GEPM(Addr)(LLVMIO))(BYTE_IMPL:ByteImpl(Addr)(LLVMIO)).
+Module MemBytesTheory(Addr:MemoryAddress.ADDRESS)(SIZEOF: Sizeof)(LLVMIO: LLVM_INTERACTIONS(Addr)(SIZEOF))(PTOI:PTOI(Addr))(PROVENANCE:PROVENANCE(Addr))(ITOP:ITOP(Addr)(PROVENANCE))(GEP:GEPM(Addr)(SIZEOF)(LLVMIO))(BYTE_IMPL:ByteImpl(Addr)(SIZEOF)(LLVMIO)).
 
   Import LLVMIO.
   Import SIZEOF.
@@ -26,7 +26,7 @@ Module MemBytesTheory(Addr:MemoryAddress.ADDRESS)(LLVMIO: LLVM_INTERACTIONS(Addr
   Import DV.
   Import GEP.
 
-  Module SER := Serialization.Make Addr LLVMIO SIZEOF PTOI PROVENANCE ITOP GEP BYTE_IMPL.
+  Module SER := Serialization.Make Addr SIZEOF LLVMIO PTOI PROVENANCE ITOP GEP BYTE_IMPL.
   Import SER.
   Import BYTE.
   Import Den.
@@ -92,22 +92,91 @@ Module MemBytesTheory(Addr:MemoryAddress.ADDRESS)(LLVMIO: LLVM_INTERACTIONS(Addr
       apply all_bytes_helper_app; eauto.
       + solve_guards_all_bytes.
   Qed.
+
+  Lemma to_ubytes_all_bytes_from_uvalue_helper :
+    forall uv dt sid sbytes,
+      is_supported dt ->
+      to_ubytes uv dt sid = sbytes ->
+      all_bytes_from_uvalue_helper 0 sid uv sbytes = Some uv.
+  Proof.  
+    intros uv dt sid sbytes SUP TO.
+
+    change 0%Z with (Z.of_N 0).
+    eapply to_ubytes_all_bytes_from_uvalue_helper'; eauto.    
+  Qed.
+
+  Lemma to_ubytes_sizeof_dtyp :
+    forall uv dt sid,  
+      N.of_nat (length (to_ubytes uv dt sid)) = sizeof_dtyp dt.
+  Proof.
+    intros uv dt sid.
+    unfold to_ubytes.
+    rewrite map_length, Nseq_length.
+    lia.
+  Qed.
+
+  Lemma from_ubytes_to_ubytes :
+    forall uv dt sid,
+      is_supported dt ->
+      sizeof_dtyp dt > 0 ->
+      from_ubytes (to_ubytes uv dt sid) dt = uv.
+  Proof.
+    intros uv dt sid SUP SIZE.
+
+    unfold from_ubytes.
+    unfold all_bytes_from_uvalue.
+
+    rewrite to_ubytes_sizeof_dtyp.
+    rewrite N.eqb_refl.
+
+    break_inner_match.
+    - (* Contradiction by size *)
+      pose proof to_ubytes_sizeof_dtyp uv dt sid.
+      rewrite Heql in H.
+
+      cbn in *.
+      lia.
+    - pose proof sbyte_to_extractbyte_inv s as (uvb & dtb & idxb & sidb & SBYTE).
+      rewrite SBYTE.
+      cbn in *.
+
+      unfold to_ubytes in Heql.
+      remember (sizeof_dtyp dt) as sz.
+      destruct sz; [inv SIZE|].
+      cbn in *.
+      pose proof Pos2Nat.is_succ p as [sz Hsz].
+      rewrite Hsz in Heql.
+      rewrite <- cons_Nseq in Heql.
+
+      cbn in Heql.
+      inv Heql.
+      rewrite sbyte_to_extractbyte_of_uvalue_sbyte in SBYTE.
+      inv SBYTE.
+      rewrite sbyte_to_extractbyte_of_uvalue_sbyte.
+      cbn.
+
+      solve_guards_all_bytes.
+
+      cbn.
+      change 1%Z with (Z.of_N 1).
+      erewrite to_ubytes_all_bytes_from_uvalue_helper'; eauto.
+  Qed.
 End MemBytesTheory.
 
-Module SerializationTheory(LLVMIO: LLVM_INTERACTIONS(Addr))(SIZEOF: Sizeof)(PTOI:PTOI(Addr))(PROVENANCE:PROVENANCE(Addr))(ITOP:ITOP(Addr)(PROVENANCE))(GEP:GEPM(Addr)(LLVMIO))(BYTE_IMPL:ByteImpl(Addr)(LLVMIO)).
+Module SerializationTheory(SIZEOF: Sizeof)(LLVMIO: LLVM_INTERACTIONS(Addr)(SIZEOF))(PTOI:PTOI(Addr))(PROVENANCE:PROVENANCE(Addr))(ITOP:ITOP(Addr)(PROVENANCE))(GEP:GEPM(Addr)(SIZEOF)(LLVMIO))(BYTE_IMPL:ByteImpl(Addr)(SIZEOF)(LLVMIO)).
 
   Import LLVMIO.
 
-  Module MBT := MemBytesTheory Addr LLVMIO SIZEOF PTOI PROVENANCE ITOP GEP BYTE_IMPL.
+  Module MBT := MemBytesTheory Addr SIZEOF LLVMIO PTOI PROVENANCE ITOP GEP BYTE_IMPL.
   Import MBT.
   Import MBT.SER.
   Import BYTE.
   Import SIZEOF.
 
-  Module Mem := FiniteMemory.Make LLVMIO PTOI PROVENANCE ITOP SIZEOF GEP BYTE_IMPL.
+  Module Mem := FiniteMemory.Make SIZEOF LLVMIO PTOI PROVENANCE ITOP GEP BYTE_IMPL.
   Export Mem.
 
-  Module ESID := ERRSID Addr LLVMIO PROVENANCE.
+  Module ESID := ERRSID Addr SIZEOF LLVMIO PROVENANCE.
   Import ESID.
 
   Lemma to_ubytes_all_bytes_from_uvalue_helper :
@@ -141,7 +210,7 @@ Module SerializationTheory(LLVMIO: LLVM_INTERACTIONS(Addr))(SIZEOF: Sizeof)(PTOI
     intros uv dt sid SUP SIZE.
 
     unfold from_ubytes.
-    unfold BYTE.all_bytes_from_uvalue.
+    unfold all_bytes_from_uvalue.
 
     rewrite to_ubytes_sizeof_dtyp.
     rewrite N.eqb_refl.
@@ -214,120 +283,510 @@ Module SerializationTheory(LLVMIO: LLVM_INTERACTIONS(Addr))(SIZEOF: Sizeof)(PTOI
   Proof.
     intros uv dt sid prov sbytes TYP SUP SIZE SER.
     induction TYP.
-    match goal with
-          (* Try easy case first for speedup *)
-          | |- _ = inr ?x =>
-            tactic_on_non_aggregate_uvalues x ltac:(cbn in SER; inv SER)
-          end;
-      cbn; rewrite from_ubytes_to_ubytes; eauto.
-    match goal with
-          (* Try easy case first for speedup *)
-          | |- _ = inr ?x =>
-            tactic_on_non_aggregate_uvalues x ltac:(cbn in SER; inv SER)
-          end;
-      cbn; rewrite from_ubytes_to_ubytes; eauto.
-    match goal with
-          (* Try easy case first for speedup *)
-          | |- _ = inr ?x =>
-            tactic_on_non_aggregate_uvalues x ltac:(cbn in SER; inv SER)
-          end;
-      cbn; rewrite from_ubytes_to_ubytes; eauto.
-    match goal with
-          (* Try easy case first for speedup *)
-          | |- _ = inr ?x =>
-            tactic_on_non_aggregate_uvalues x ltac:(cbn in SER; inv SER)
-          end;
-      cbn; rewrite from_ubytes_to_ubytes; eauto.
-    match goal with
-          (* Try easy case first for speedup *)
-          | |- _ = inr ?x =>
-            tactic_on_non_aggregate_uvalues x ltac:(cbn in SER; inv SER)
-          end;
-      cbn; rewrite from_ubytes_to_ubytes; eauto.
-    match goal with
-          (* Try easy case first for speedup *)
-          | |- _ = inr ?x =>
-            tactic_on_non_aggregate_uvalues x ltac:(cbn in SER; inv SER)
-          end;
-      cbn; rewrite from_ubytes_to_ubytes; eauto.
+(*     match goal with *)
+(*           (* Try easy case first for speedup *) *)
+(*           | |- _ = inr ?x => *)
+(*             tactic_on_non_aggregate_uvalues x ltac:(cbn in SER; inv SER) *)
+(*           end; *)
+(*       cbn; rewrite from_ubytes_to_ubytes; eauto. *)
+(*     match goal with *)
+(*           (* Try easy case first for speedup *) *)
+(*           | |- _ = inr ?x => *)
+(*             tactic_on_non_aggregate_uvalues x ltac:(cbn in SER; inv SER) *)
+(*           end; *)
+(*       cbn; rewrite from_ubytes_to_ubytes; eauto. *)
+(*     match goal with *)
+(*           (* Try easy case first for speedup *) *)
+(*           | |- _ = inr ?x => *)
+(*             tactic_on_non_aggregate_uvalues x ltac:(cbn in SER; inv SER) *)
+(*           end; *)
+(*       cbn; rewrite from_ubytes_to_ubytes; eauto. *)
+(*     match goal with *)
+(*           (* Try easy case first for speedup *) *)
+(*           | |- _ = inr ?x => *)
+(*             tactic_on_non_aggregate_uvalues x ltac:(cbn in SER; inv SER) *)
+(*           end; *)
+(*       cbn; rewrite from_ubytes_to_ubytes; eauto. *)
+(*     match goal with *)
+(*           (* Try easy case first for speedup *) *)
+(*           | |- _ = inr ?x => *)
+(*             tactic_on_non_aggregate_uvalues x ltac:(cbn in SER; inv SER) *)
+(*           end; *)
+(*       cbn; rewrite from_ubytes_to_ubytes; eauto. *)
+(*     match goal with *)
+(*           (* Try easy case first for speedup *) *)
+(*           | |- _ = inr ?x => *)
+(*             tactic_on_non_aggregate_uvalues x ltac:(cbn in SER; inv SER) *)
+(*           end; *)
+(*       cbn; rewrite from_ubytes_to_ubytes; eauto. *)
 
-    - unfold deserialize_sbytes.
-      cbn.
-cbn in *;
-        destruct t.
-      cbn.
-      reflexivity.
-      destruct t.
+(*     - unfold deserialize_sbytes. *)
+(*       cbn. *)
+(* cbn in *; *)
+(*         destruct t. *)
+(*       cbn *)
+(*       reflexivity. *)
+(*       destruct t. *)
 
-      cbn; inv SER.
-          rewrite from_ubytes_to_ubytes; eauto.
-
-
-
-    solve [match goal with
-          (* Try easy case first for speedup *)
-          | |- _ = inr ?x =>
-            tactic_on_non_aggregate_uvalues x ltac:(cbn in SER; inv SER)
-          end;
-      cbn; rewrite from_ubytes_to_ubytes; eauto].
-    match goal with
-          (* Try easy case first for speedup *)
-          | |- _ = inr ?x =>
-            tactic_on_non_aggregate_uvalues x ltac:(cbn in SER; inv SER)
-          end;
-      cbn; rewrite from_ubytes_to_ubytes; eauto.
-    match goal with
-          (* Try easy case first for speedup *)
-          | |- _ = inr ?x =>
-            tactic_on_non_aggregate_uvalues x ltac:(cbn in SER; inv SER)
-          end;
-      cbn; rewrite from_ubytes_to_ubytes; eauto.
-    match goal with
-          (* Try easy case first for speedup *)
-          | |- _ = inr ?x =>
-            tactic_on_non_aggregate_uvalues x ltac:(cbn in SER; inv SER)
-          end;
-      cbn; rewrite from_ubytes_to_ubytes; eauto.
-    match goal with
-          (* Try easy case first for speedup *)
-          | |- _ = inr ?x =>
-            tactic_on_non_aggregate_uvalues x ltac:(cbn in SER; inv SER)
-          end;
-      cbn; rewrite from_ubytes_to_ubytes; eauto.
-    match goal with
-          (* Try easy case first for speedup *)
-          | |- _ = inr ?x =>
-            tactic_on_non_aggregate_uvalues x ltac:(cbn in SER; inv SER)
-          end;
-      cbn; rewrite from_ubytes_to_ubytes; eauto.
+(*       cbn; inv SER. *)
+(*           rewrite from_ubytes_to_ubytes; eauto. *)
 
 
-    49: { eval_serialize_sbytes_hyp.
-    56: { cbn in SER. destruct bytes. cbn in *. }
-    all:eval_serialize_sbytes_hyp.
-    1-30:eval_serialize_sbytes_hyp.
-    12: {
-      eval_serialize_sbytes_hyp.
+
+(*     solve [match goal with *)
+(*           (* Try easy case first for speedup *) *)
+(*           | |- _ = inr ?x => *)
+(*             tactic_on_non_aggregate_uvalues x ltac:(cbn in SER; inv SER) *)
+(*           end; *)
+(*       cbn; rewrite from_ubytes_to_ubytes; eauto]. *)
+(*     match goal with *)
+(*           (* Try easy case first for speedup *) *)
+(*           | |- _ = inr ?x => *)
+(*             tactic_on_non_aggregate_uvalues x ltac:(cbn in SER; inv SER) *)
+(*           end; *)
+(*       cbn; rewrite from_ubytes_to_ubytes; eauto. *)
+(*     match goal with *)
+(*           (* Try easy case first for speedup *) *)
+(*           | |- _ = inr ?x => *)
+(*             tactic_on_non_aggregate_uvalues x ltac:(cbn in SER; inv SER) *)
+(*           end; *)
+(*       cbn; rewrite from_ubytes_to_ubytes; eauto. *)
+(*     match goal with *)
+(*           (* Try easy case first for speedup *) *)
+(*           | |- _ = inr ?x => *)
+(*             tactic_on_non_aggregate_uvalues x ltac:(cbn in SER; inv SER) *)
+(*           end; *)
+(*       cbn; rewrite from_ubytes_to_ubytes; eauto. *)
+(*     match goal with *)
+(*           (* Try easy case first for speedup *) *)
+(*           | |- _ = inr ?x => *)
+(*             tactic_on_non_aggregate_uvalues x ltac:(cbn in SER; inv SER) *)
+(*           end; *)
+(*       cbn; rewrite from_ubytes_to_ubytes; eauto. *)
+(*     match goal with *)
+(*           (* Try easy case first for speedup *) *)
+(*           | |- _ = inr ?x => *)
+(*             tactic_on_non_aggregate_uvalues x ltac:(cbn in SER; inv SER) *)
+(*           end; *)
+(*       cbn; rewrite from_ubytes_to_ubytes; eauto. *)
+
+
+(*     49: { eval_serialize_sbytes_hyp. *)
+(*     56: { cbn in SER. destruct bytes. cbn in *. } *)
+(*     all:eval_serialize_sbytes_hyp. *)
+(*     1-30:eval_serialize_sbytes_hyp. *)
+(*     12: { *)
+(*       eval_serialize_sbytes_hyp. *)
       
-      rewrite serialize_sbytes_equation in SER.
-    }
-    rewrite serialize_sbytes_equation in SER.
-      try solve [cbn in SER; inv SER; cbn; rewrite from_ubytes_to_ubytes; eauto].
+(*       rewrite serialize_sbytes_equation in SER. *)
+(*     } *)
+(*     rewrite serialize_sbytes_equation in SER. *)
+(*       try solve [cbn in SER; inv SER; cbn; rewrite from_ubytes_to_ubytes; eauto]. *)
 
     
-    induction TYP;
-      try solve [unfold serialize_sbytes in SER;
-                 inv SER;
-                 unfold deserialize_sbytes;
-                 rewrite from_ubytes_to_ubytes; eauto
-                | cbn in *;
-                  match goal with
-                  | |- deserialize_sbytes _ ?t = _ =>
-                    cbn in *;
-                    destruct t; cbn; inv SER;
-                    rewrite from_ubytes_to_ubytes; eauto
-                  end
-                ].
-    - inv SUP; exfalso; apply H; constructor.
-    - rewrite sizeof_dtyp_void in SIZE. inv SIZE.
-  Qed.
+(*     induction TYP; *)
+(*       try solve [unfold serialize_sbytes in SER; *)
+(*                  inv SER; *)
+(*                  unfold deserialize_sbytes; *)
+(*                  rewrite from_ubytes_to_ubytes; eauto *)
+(*                 | cbn in *; *)
+(*                   match goal with *)
+(*                   | |- deserialize_sbytes _ ?t = _ => *)
+(*                     cbn in *; *)
+(*                     destruct t; cbn; inv SER; *)
+(*                     rewrite from_ubytes_to_ubytes; eauto *)
+(*                   end *)
+(*                 ]. *)
+(*     - inv SUP; exfalso; apply H; constructor. *)
+(*     - rewrite sizeof_dtyp_void in SIZE. inv SIZE. *)
+(*   Qed. *)
+  Admitted.
+
+    (** ** Deserialize - Serialize
+        Starting from a dvalue [val] whose [dtyp] is [t], if:
+        1. we serialize [val], getting a [list SByte]
+        2. we add all these bytes to the memory block, starting from the position [off], getting back a new [mem_block] m'
+        3. we lookup in this new memory [m'] the indices starting from [off] for the size of [t], getting back a [list SByte]
+        4. we deserialize this final list of bytes
+        then we should get back the initial value [val], albeit injected into [uvalue].
+
+        The proof should go by induction over [TYP] I think, and rely on [lookup_all_index_add] notably.
+     *)
+    Lemma deserialize_serialize : forall val dt sid prov bytes,
+        uvalue_has_dtyp val dt ->
+        ErrSID_evals_to (serialize_sbytes val dt) bytes sid prov ->
+        deserialize_sbytes bytes dt = inr val.
+    Proof.
+      intros val dt sid prov bytes TYP SER.
+      induction TYP.
+      - cbn in SER; inv SER.
+        cbn.
+    Admitted.
+
+    (* Lemma deserialize_serialize : forall val t (TYP : dvalue_has_dtyp val t), *)
+    (*     forall off (bytes : mem_block) (SUP : is_supported t), *)
+    (*       deserialize_sbytes (lookup_all_index off (sizeof_dtyp t) (add_all_index (serialize_dvalue val) off bytes) SUndef) t = dvalue_to_uvalue val. *)
+    (* Proof. *)
+    (*   induction 1; try auto; intros; *)
+    (*     match goal with *)
+    (*     | H: is_supported ?t |- _ => *)
+    (*       try solve [inversion H] *)
+    (*     end. *)
+    (*   - unroll_lookup_all_index; cbn; f_equal. *)
+    (*   - unroll_lookup_all_index; cbn; f_equal. *)
+    (*     pose proof (unsigned_I1_in_range x). *)
+    (*     assert (EQ :DynamicValues.Int1.unsigned x / 256 = 0). *)
+    (*     apply Z.div_small; lia. *)
+    (*     rewrite EQ. *)
+    (*     repeat rewrite Zdiv_0_l. *)
+    (*     repeat rewrite Byte.unsigned_repr. *)
+    (*     all: unfold Byte.max_unsigned, Byte.modulus; cbn; try lia. *)
+    (*     rewrite Z.add_0_r. *)
+    (*     apply DynamicValues.Int1.repr_unsigned. *)
+    (*   - solve_integer_deserialize. *)
+    (*   - solve_integer_deserialize. *)
+    (*   - solve_integer_deserialize. *)
+    (*   - inversion SUP; subst; *)
+    (*     exfalso; apply H; constructor. *)
+    (*   - unroll_lookup_all_index; cbn; f_equal. *)
+    (*     clear bytes off. *)
+    (*     remember (Float.to_bits x) as xb. *)
+    (*     pose proof (unsigned_I64_in_range xb). *)
+    (*     repeat rewrite Byte.unsigned_repr_eq. *)
+    (*     unfold Byte.modulus, Byte.wordsize, Wordsize_8.wordsize; cbn. *)
+    (*     replace (two_power_nat 8) with 256 by reflexivity. *)
+    (*     remember (Int64.unsigned xb) as xbv. *)
+    (*     match goal with *)
+    (*     | [|- context[Int64.repr ?zv]] => replace zv with xbv *)
+    (*     end. *)
+    (*     + *)
+    (*       subst. *)
+    (*       rewrite Int64.repr_unsigned. *)
+    (*       apply Float.of_to_bits. *)
+    (*     + *)
+    (*       (* this is the same goal as I64 branch! *) *)
+    (*       clear -H. *)
+    (*       rewrite Z.add_0_r. *)
+    (*       unfold Z.modulo. *)
+    (*       repeat break_let. *)
+    (*       repeat match goal with *)
+    (*              | [H : Z.div_eucl _ _ = _ |- _] => apply Z_div_mod' in H; [destruct H | lia] *)
+    (*              end. *)
+    (*       subst. *)
+    (*       repeat *)
+    (*         match goal with *)
+    (*         | H: context [(?d * ?x + ?z) / ?d] |- _ => *)
+    (*           rewrite div_add_lemma in H; [|lia]; subst *)
+    (*         end. *)
+    (*       lia. *)
+    (*   - unroll_lookup_all_index; cbn; f_equal. *)
+    (*     clear bytes off. *)
+    (*     remember (Float32.to_bits x) as xb. *)
+    (*     pose proof (unsigned_I32_in_range xb). *)
+    (*     repeat rewrite Byte.unsigned_repr_eq. *)
+    (*     unfold Byte.modulus, Byte.wordsize, Wordsize_8.wordsize; cbn. *)
+    (*     replace (two_power_nat 8) with 256 by reflexivity. *)
+    (*     remember (Int32.unsigned xb) as xbv. *)
+    (*     match goal with *)
+    (*     | [|- context[Int32.repr ?zv]] => replace zv with xbv *)
+    (*     end. *)
+    (*     + *)
+    (*       subst. *)
+    (*       rewrite Int32.repr_unsigned. *)
+    (*       apply Float32.of_to_bits. *)
+    (*     + *)
+    (*       clear -H. *)
+
+    (*       rewrite Z.add_0_r. *)
+    (*       unfold Z.modulo. *)
+    (*       repeat break_let. *)
+    (*       repeat match goal with *)
+    (*              | [H : Z.div_eucl _ _ = _ |- _] => apply Z_div_mod' in H; [destruct H | lia] *)
+    (*              end. *)
+    (*       subst. *)
+    (*       rewrite Z.add_comm, Z.mul_comm, Z_div_plus in * by lia. *)
+    (*       rewrite Zdiv_small with (x:=z0) in * by lia. *)
+    (*       rewrite Z.add_0_l in *. *)
+    (*       subst. *)
+    (*       rewrite Z.add_comm, Z.mul_comm, Z_div_plus in * by lia. *)
+    (*       rewrite Zdiv_small with (x:=z2) in * by lia. *)
+    (*       rewrite Z.add_0_l in *. *)
+    (*       subst. *)
+    (*       rewrite Z.add_comm, Z.mul_comm, Z_div_plus in * by lia. *)
+    (*       rewrite Zdiv_small with (x:=z4) in * by lia. *)
+    (*       rewrite Z.add_0_l in *. *)
+    (*       subst. *)
+    (*       lia. *)
+    (*   - (* Structs *) *)
+    (*     rewrite sizeof_struct_cons. *)
+
+    (*     inversion SUP. *)
+    (*     subst. *)
+    (*     rename H0 into FIELD_SUP. *)
+    (*     apply List.Forall_cons_iff in FIELD_SUP. *)
+    (*     destruct FIELD_SUP as [dt_SUP dts_SUP]. *)
+    (*     assert (is_supported (DTYPE_Struct dts)) as SUP_STRUCT by (constructor; auto). *)
+
+    (*     cbn. *)
+    (*     rewrite lookup_all_index_append; [|apply sizeof_serialized; auto]. *)
+
+    (*     erewrite deserialize_struct_element; auto. *)
+    (*     +  erewrite <- sizeof_serialized; eauto. *)
+    (*       rewrite lookup_all_index_add_all_index_same_length; eauto. *)
+
+    (*       apply dvalue_serialized_not_sundef. *)
+    (*     + pose proof deserialize_sbytes_dvalue_all_not_sundef (DVALUE_Struct fields) (DTYPE_Struct dts) (lookup_all_index (off + Z.of_N (sizeof_dtyp dt)) (sizeof_dtyp (DTYPE_Struct dts)) *)
+    (*                                                                                                                       (add_all_index (serialize_dvalue (DVALUE_Struct fields)) (off + Z.of_N (sizeof_dtyp dt)) bytes) SUndef). *)
+    (*       cbn in H. *)
+    (*       forward H; auto. *)
+    (*     + rewrite lookup_all_index_length. *)
+    (*       reflexivity. *)
+    (*   - (* Packed structs *) *)
+    (*     rewrite sizeof_packed_struct_cons. *)
+
+    (*     inversion SUP. *)
+    (*     subst. *)
+    (*     rename H0 into FIELD_SUP. *)
+    (*     apply List.Forall_cons_iff in FIELD_SUP. *)
+    (*     destruct FIELD_SUP as [dt_SUP dts_SUP]. *)
+    (*     assert (is_supported (DTYPE_Packed_struct dts)) as SUP_STRUCT by (constructor; auto). *)
+
+    (*     cbn. *)
+    (*     rewrite lookup_all_index_append; [|apply sizeof_serialized; auto]. *)
+
+    (*     erewrite deserialize_packed_struct_element; auto. *)
+    (*     + erewrite <- sizeof_serialized; eauto. *)
+    (*       rewrite lookup_all_index_add_all_index_same_length; eauto. *)
+
+    (*       apply dvalue_serialized_not_sundef. *)
+    (*     + pose proof deserialize_sbytes_dvalue_all_not_sundef (DVALUE_Packed_struct fields) (DTYPE_Packed_struct dts) (lookup_all_index (off + Z.of_N (sizeof_dtyp dt)) (sizeof_dtyp (DTYPE_Packed_struct dts)) *)
+    (*                                                                                                                       (add_all_index (serialize_dvalue (DVALUE_Packed_struct fields)) (off + Z.of_N (sizeof_dtyp dt)) bytes) SUndef). *)
+    (*       cbn in H. *)
+    (*       forward H; auto. *)
+    (*     + rewrite lookup_all_index_length. *)
+    (*       reflexivity. *)
+    (*   - (* Arrays *) *)
+    (*     rename H into SZ. *)
+    (*     generalize dependent sz. *)
+    (*     generalize dependent xs. *)
+    (*     induction xs; *)
+    (*       intros IH IHdtyp sz SZ SUP. *)
+    (*     + cbn in *. *)
+    (*       subst. *)
+    (*       reflexivity. *)
+    (*     + cbn in SZ. *)
+    (*       subst. *)
+    (*       rewrite Nnat.Nat2N.inj_succ. *)
+    (*       cbn. *)
+
+    (*       assert (dvalue_has_dtyp a dt) as DTa. *)
+    (*       { *)
+    (*         apply IHdtyp. *)
+    (*         cbn. auto. *)
+    (*       } *)
+
+    (*       rewrite Nmult_Sn_m. *)
+    (*       rewrite lookup_all_index_append; [|apply sizeof_serialized; auto]. *)
+
+    (*       erewrite deserialize_array_element; auto. *)
+    (*       * inversion SUP; constructor; auto. *)
+    (*       * erewrite <- sizeof_serialized; eauto. *)
+    (*         rewrite lookup_all_index_add_all_index_same_length; eauto. *)
+
+    (*         apply dvalue_serialized_not_sundef. *)
+    (*       * (* Should be serialization of DVALUE_array xs *) *)
+    (*         replace (N.of_nat (Datatypes.length xs) * sizeof_dtyp dt)%N *)
+    (*           with (N.of_nat (N.to_nat (N.of_nat (Datatypes.length xs) * sizeof_dtyp dt))) by lia. *)
+    (*         rewrite lookup_all_index_add_all_index_same_length. *)
+
+    (*         apply all_not_sundef_fold_right_serialize. *)
+
+    (*         apply serialize_fold_length; intuition. *)
+    (*       * replace (sizeof_dtyp dt) with (N.of_nat (N.to_nat (sizeof_dtyp dt))) by lia. *)
+    (*         rewrite lookup_all_index_add_all_index_same_length. *)
+    (*         erewrite <- sizeof_serialized; intuition. *)
+    (*         lia. *)
+    (*         erewrite <- sizeof_serialized; intuition. *)
+    (*         lia. *)
+    (*       * rewrite IH; intuition. *)
+    (*         inversion SUP; auto. *)
+    (*       * cbn. *)
+
+    (*         unfold deserialize_sbytes. *)
+    (*         break_match. *)
+
+    (*         2: { *)
+    (*           assert (all_not_sundef *)
+    (*                     (lookup_all_index (off + Z.of_N (sizeof_dtyp dt)) *)
+    (*                                       (N.of_nat (Datatypes.length xs) * sizeof_dtyp dt) *)
+    (*                                       (add_all_index *)
+    (*                                          (fold_right (fun (dv : dvalue) (acc : list SByte) => serialize_dvalue dv ++ acc) [] *)
+    (*                                                      xs) (off + Z.of_N (sizeof_dtyp dt)) bytes) SUndef) = true) as CONTRA. *)
+    (*           replace (N.of_nat (Datatypes.length xs) * sizeof_dtyp dt)%N *)
+    (*             with (N.of_nat (N.to_nat (N.of_nat (Datatypes.length xs) * sizeof_dtyp dt))) by lia. *)
+    (*           rewrite lookup_all_index_add_all_index_same_length. *)
+
+    (*           apply all_not_sundef_fold_right_serialize. *)
+
+    (*           apply serialize_fold_length; intuition. *)
+
+    (*           rewrite Heqb in CONTRA. *)
+    (*           inversion CONTRA. *)
+    (*         } *)
+
+    (*         forward IHxs; intuition. *)
+    (*         forward IHxs; intuition. *)
+    (*         specialize (IHxs (Datatypes.length xs) eq_refl). *)
+    (*         forward IHxs. *)
+    (*         { inversion SUP; constructor; eauto. } *)
+
+    (*         cbn in IHxs. *)
+    (*         rewrite <- IHxs. *)
+
+    (*         rewrite all_not_sundef_deserialized; auto. *)
+    (*         erewrite <- sizeof_serialized. *)
+
+    (*         f_equal. *)
+
+    (*         repeat rewrite <- Nnat.Nat2N.inj_mul. *)
+    (*         rewrite lookup_all_index_add_all_index_same_length. *)
+    (*         rewrite lookup_all_index_add_all_index_same_length. *)
+    (*         reflexivity. *)
+
+    (*         { erewrite <- serialize_fold_length. *)
+    (*           erewrite <- sizeof_serialized. *)
+
+    (*           repeat rewrite <- Nnat.Nat2N.inj_mul. *)
+    (*           rewrite Nnat.Nat2N.id. *)
+    (*           reflexivity. *)
+
+    (*           eauto. *)
+    (*           intuition. *)
+    (*         } *)
+
+    (*         { erewrite <- serialize_fold_length. *)
+    (*           erewrite <- sizeof_serialized. *)
+
+    (*           repeat rewrite <- Nnat.Nat2N.inj_mul. *)
+    (*           rewrite Nnat.Nat2N.id. *)
+    (*           reflexivity. *)
+
+    (*           eauto. *)
+    (*           intuition. *)
+    (*         } *)
+
+    (*         eauto. *)
+    (*   - (* Vectors *) *)
+    (*     rename H into SZ. *)
+    (*     generalize dependent sz. *)
+    (*     generalize dependent xs. *)
+    (*     induction xs; *)
+    (*       intros IH IHdtyp sz SZ SUP. *)
+    (*     + cbn in *. *)
+    (*       subst. *)
+    (*       reflexivity. *)
+    (*     + cbn in SZ. *)
+    (*       subst. *)
+    (*       rewrite Nnat.Nat2N.inj_succ. *)
+    (*       cbn. *)
+
+    (*       assert (dvalue_has_dtyp a dt) as DTa. *)
+    (*       { *)
+    (*         apply IHdtyp. *)
+    (*         cbn. auto. *)
+    (*       } *)
+
+    (*       rewrite Nmult_Sn_m. *)
+    (*       rewrite lookup_all_index_append; [|apply sizeof_serialized; auto]. *)
+
+    (*       erewrite deserialize_vector_element; auto. *)
+    (*       * inversion SUP; constructor; auto. *)
+    (*       * erewrite <- sizeof_serialized; eauto. *)
+    (*         rewrite lookup_all_index_add_all_index_same_length; eauto. *)
+
+    (*         apply dvalue_serialized_not_sundef. *)
+    (*       * (* Should be serialization of DVALUE_vector xs *) *)
+    (*         replace (N.of_nat (Datatypes.length xs) * sizeof_dtyp dt)%N *)
+    (*           with (N.of_nat (N.to_nat (N.of_nat (Datatypes.length xs) * sizeof_dtyp dt))) by lia. *)
+    (*         rewrite lookup_all_index_add_all_index_same_length. *)
+
+    (*         apply all_not_sundef_fold_right_serialize. *)
+
+    (*         apply serialize_fold_length; intuition. *)
+    (*       * replace (sizeof_dtyp dt) with (N.of_nat (N.to_nat (sizeof_dtyp dt))) by lia. *)
+    (*         rewrite lookup_all_index_add_all_index_same_length. *)
+    (*         erewrite <- sizeof_serialized; intuition. *)
+    (*         lia. *)
+    (*         erewrite <- sizeof_serialized; intuition. *)
+    (*         lia. *)
+    (*       * rewrite IH; intuition. *)
+    (*         inversion SUP; subst; auto. *)
+    (*       * cbn. *)
+
+    (*         unfold deserialize_sbytes. *)
+    (*         break_match. *)
+
+    (*         2: { *)
+    (*           assert (all_not_sundef *)
+    (*                     (lookup_all_index (off + Z.of_N (sizeof_dtyp dt)) *)
+    (*                                       (N.of_nat (Datatypes.length xs) * sizeof_dtyp dt) *)
+    (*                                       (add_all_index *)
+    (*                                          (fold_right (fun (dv : dvalue) (acc : list SByte) => serialize_dvalue dv ++ acc) [] *)
+    (*                                                      xs) (off + Z.of_N (sizeof_dtyp dt)) bytes) SUndef) = true) as CONTRA. *)
+    (*           replace (N.of_nat (Datatypes.length xs) * sizeof_dtyp dt)%N *)
+    (*             with (N.of_nat (N.to_nat (N.of_nat (Datatypes.length xs) * sizeof_dtyp dt))) by lia. *)
+    (*           rewrite lookup_all_index_add_all_index_same_length. *)
+
+    (*           apply all_not_sundef_fold_right_serialize. *)
+
+    (*           apply serialize_fold_length; intuition. *)
+
+    (*           rewrite Heqb in CONTRA. *)
+    (*           inversion CONTRA. *)
+    (*         } *)
+
+    (*         forward IHxs; intuition. *)
+    (*         forward IHxs; intuition. *)
+    (*         specialize (IHxs (Datatypes.length xs) eq_refl). *)
+    (*         forward IHxs. *)
+    (*         { inversion SUP; constructor; eauto. } *)
+
+    (*         cbn in IHxs. *)
+    (*         rewrite <- IHxs. *)
+
+    (*         rewrite all_not_sundef_deserialized; auto. *)
+    (*         erewrite <- sizeof_serialized. *)
+
+    (*         f_equal. *)
+
+    (*         repeat rewrite <- Nnat.Nat2N.inj_mul. *)
+    (*         rewrite lookup_all_index_add_all_index_same_length. *)
+    (*         rewrite lookup_all_index_add_all_index_same_length. *)
+    (*         reflexivity. *)
+
+    (*         { erewrite <- serialize_fold_length. *)
+    (*           erewrite <- sizeof_serialized. *)
+
+    (*           repeat rewrite <- Nnat.Nat2N.inj_mul. *)
+    (*           rewrite Nnat.Nat2N.id. *)
+    (*           reflexivity. *)
+
+    (*           eauto. *)
+    (*           intuition. *)
+    (*         } *)
+
+    (*         { erewrite <- serialize_fold_length. *)
+    (*           erewrite <- sizeof_serialized. *)
+
+    (*           repeat rewrite <- Nnat.Nat2N.inj_mul. *)
+    (*           rewrite Nnat.Nat2N.id. *)
+    (*           reflexivity. *)
+
+    (*           eauto. *)
+    (*           intuition. *)
+    (*         } *)
+
+    (*         eauto. *)
+    (* Qed. *)
+
+End SerializationTheory.
